
\documentclass[tikz,border=10pt]{standalone}


\RequirePackage{luatex85}
\usepackage[utf8]{inputenc}
\usepackage{amsmath, amssymb, amsfonts, accents}
\usetikzlibrary{graphdrawing, graphs, arrows, shapes, automata, calc}
\usepackage{stix}

% workaround for https://github.com/u-fischer/luaotfload/issues/6
\usepackage{luacode}
\begin{luacode}
  function pgf_lookup_and_require(name)
    local sep = '/'
    if string.find(os.getenv('PATH'),';') then
      sep = '\string\\'
    end
    local function lookup(name)
      local sub = name:gsub('%.',sep)
      local find_func = function (name, suffix)
        if resolvers then
          local n = resolvers.findfile (name.."."..suffix, suffix) -- changed
          return (not (n == '')) and n or nil
        else
          return kpse.find_file(name,suffix)
        end
      end
      if find_func(sub, 'lua') then
        require(name)
      elseif find_func(sub, 'clua') then
        collectgarbage('stop')
        require(name)
        collectgarbage('restart')
      else
        return false
      end
      return true
    end
    return
      lookup('pgf.gd.' .. name .. '.library') or
      lookup('pgf.gd.' .. name) or
      lookup(name .. '.library') or
      lookup(name)
  end
\end{luacode}
\usegdlibrary{trees, layered}


\newcommand{\Xund}{\rule{.4em}{.4pt}}
\newcommand{\IRE}{I\!RE}


\begin{document}

\begin{tikzpicture}[>=stealth, ->, auto, node distance=0.2in]

\tikzstyle{every node}=[draw=none, shape=rectangle, outer sep = 0in];

\small{

\begin{scope}[xshift=-0in, yshift=0in]
    \node (a) {{
    $\begin{aligned}
        & mark (1,\; (((\epsilon|a^{0,\infty}))(\epsilon|a)^{0,3} )) = \big[ \\[-0.2em]
        & \quad mark (2,\; ((\epsilon|a^{0,\infty}))(\epsilon|a)^{0,\infty} ) = \big[ \\[-0.2em]
        %
        & \quad\quad mark (2,\; ((\epsilon|a^{0,\infty})) ) = \big[ \\[-0.2em]
        & \quad\quad\quad mark (3,\; (\epsilon|a^{0,\infty}) ) = \big[ \\[-0.2em]
        & \quad\quad\quad\quad mark (4,\; \epsilon|a^{0,\infty} ) = \big[ \\[-0.2em]
        & \quad\quad\quad\quad\quad mark (4,\; \epsilon ) = (4,\; (0,\emptyset,\epsilon)) \\[-0.2em]
        & \quad\quad\quad\quad\quad mark (4,\; a^{0,\infty} ) = \big[ \\[-0.2em]
        & \quad\quad\quad\quad\quad\quad mark (4,\; a ) = (4,\; (0,\emptyset,a)) \\[-0.2em]
        & \quad\quad\quad\quad\quad \big] = (4,\; (0,\emptyset,(0,\emptyset,a)^{0,\infty})) \\[-0.2em]
        & \quad\quad\quad\quad \big] = (4,\; (0,\emptyset,(0,\emptyset,\epsilon) \mid (0,\emptyset,(0,\emptyset,a)^{0,\infty}))) \\[-0.2em]
        & \quad\quad\quad \big] = (4,\; (1,\{3\},(0,\emptyset,\epsilon) \mid (0,\emptyset,(0,\emptyset,a)^{0,\infty}))) \\[-0.2em]
        & \quad\quad \big] = (4,\; (1,\{2, 3\},(0,\emptyset,\epsilon) \mid (0,\emptyset,(0,\emptyset,a)^{0,\infty}))) \\[-0.2em]
        %
        & \quad\quad mark (4,\; (\epsilon|a)^{0,3} ) = \big[ \\[-0.2em]
        & \quad\quad\quad mark (4,\; (\epsilon|a) ) = \big[ \\[-0.2em]
        & \quad\quad\quad\quad mark (5,\; \epsilon|a ) = \big [ \\[-0.2em]
        & \quad\quad\quad\quad\quad mark (5,\; \epsilon ) = (5,\; (0,\emptyset,\epsilon)) \\[-0.2em]
        & \quad\quad\quad\quad\quad mark (5,\; a ) = (5,\; (0,\emptyset,a)) \\[-0.2em]
        & \quad\quad\quad\quad \big] = (5,\; (0,\emptyset,(0,\emptyset,\epsilon) \mid (0,\emptyset,a))) \\[-0.2em]
        & \quad\quad\quad \big] = (5,\; (1,\{4\},(0,\emptyset,\epsilon) \mid (0,\emptyset,a))) \\[-0.2em]
        & \quad\quad \big] = (5,\; (1,\emptyset,(1,\{4\},(0,\emptyset,\epsilon) \mid (0,\emptyset,a))^{0,3})) \\[-0.2em]
        %
        & \quad\big] = (5,\; (1,\emptyset,
           (1,\{2,3\},(0,\emptyset,\epsilon) \mid (0,\emptyset,(0,\emptyset,a)^{0,\infty})) \\[-0.2em]
           & \quad\quad\quad\quad\quad\enspace \cdot (1,\emptyset,(1,\{4\},(0,\emptyset,\epsilon) \mid (0,\emptyset,a))^{0,3})
           )) \\[-0.2em]
        & \big] = (5,\; (1,\{1\},
           (1,\{2,3\},(0,\emptyset,\epsilon) \mid (0,\emptyset,(0,\emptyset,a)^{0,\infty})) \\[-0.2em]
           & \quad\quad\quad\quad\quad\enspace \cdot (1,\emptyset,(1,\{4\},(0,\emptyset,\epsilon) \mid (0,\emptyset,a))^{0,3})
           ))
    \end{aligned}$
    }};
\end{scope}

\begin{scope}[xshift=0in, yshift=-3.9in]
    \node (a) {{
    $\begin{aligned}
        & enum (1,\; (1,\{1\},
            (1,\{2,3\},(0,\emptyset,\epsilon) \mid (0,\emptyset,(0,\emptyset,a)^{0,\infty})) \\[-0.2em]
            & \quad\quad\quad\quad\quad\quad \cdot (1,\emptyset,(1,\{4\},(0,\emptyset,\epsilon) \mid (0,\emptyset,a))^{0,\infty}))) = \big[ \\[-0.2em]
        & \quad enum (2,\; (1,\{2,3\},(0,\emptyset,\epsilon) \mid (0,\emptyset,(0,\emptyset,a)^{0,\infty}))) = \big[ \\[-0.2em]
        & \quad\quad enum (3,\; (0,\emptyset,\epsilon)) = (3,\; (0,\emptyset,\epsilon)) \\[-0.2em]
        & \quad\quad enum (3,\; (0,\emptyset,(0,\emptyset,a)^{0,\infty})) = \big[ \\[-0.2em]
        & \quad\quad\quad enum (3,\; (0,\emptyset,a)) = (3,\; (0,\emptyset,a)) \\[-0.2em]
        & \quad\quad \big] = (3,\; (0,\emptyset,(0,\emptyset,a)^{0,\infty})) \\[-0.2em]
        & \quad \big] = (3,\; (2,\{2,3\},(0,\emptyset,\epsilon) \mid (0,\emptyset,(0,\emptyset,a)^{0,\infty}))) \\[-0.2em]
        %
        & \quad enum (3,\; (1,\emptyset,(1,\{4\},(0,\emptyset,\epsilon) \mid (0,\emptyset,a))^{0,\infty}) ) = \big[ \\[-0.2em]
        & \quad\quad enum (4,\; (1,\{4\},(0,\emptyset,\epsilon) \mid (0,\emptyset,a)) ) = \big[ \\[-0.2em]
        & \quad\quad\quad enum (5,\; (0,\emptyset,\epsilon) ) = (5,\; (0,\emptyset,\epsilon)) \\[-0.2em]
        & \quad\quad\quad enum (5,\; (0,\emptyset,a) ) = (5,\; (0,\emptyset,a)) \\[-0.2em]
        & \quad\quad \big] = (5,\; (4,\{4\},(0,\emptyset,\epsilon) \mid (0,\emptyset,a))) \\[-0.2em]
        & \quad \big] = (5,\; (3,\emptyset,(4,\{4\},(0,\emptyset,\epsilon) \mid (0,\emptyset,a))^{0,\infty})) \\[-0.2em]
        %
        & \big] = (5,\; (1,\{1\},
            (2,\{2,3\},(0,\emptyset,\epsilon) \mid (0,\emptyset,(0,\emptyset,a)^{0,\infty})) \\[-0.2em]
            & \quad\quad\quad\quad\quad\enspace \cdot (3,\emptyset,(4,\{4\},(0,\emptyset,\epsilon) \mid (0,\emptyset,a))^{0,\infty})
            ))
    \end{aligned}$
    }};
\end{scope}

\begin{scope}[xshift=3in, yshift=2.1in]
    \graph [tree layout, grow=down, fresh nodes, level distance=0.35in] {
        "${(1, \{1\}, Cat)}_{\Lambda}$" -- {
            "${(2, \{2,3\}, Alt)}_{1}$" -- {
                "${(0, \emptyset, \epsilon)}_{1.1}$",
                "${(0, \emptyset, Rep(0,\infty))}_{1.2}$" -- {
                    "${(0, \emptyset, a)}_{1.2.1}$"
                }
            },
            "$({3, \emptyset, Rep(0,3))}_{2}$" -- {
                "${(4, \{4\}, Alt)}_{2.1}$" -- {
                    "${(0, \emptyset, a)}_{2.1.1}$",
                    "${(0, \emptyset, \epsilon)}_{2.1.2}$"
                }
            }
        }
    };
\end{scope}

\begin{scope}[xshift=3in, yshift=0.5in]
    \node (c) {{
    $\begin{aligned}
        & I\!RE\big( (((\epsilon|a^{0,\infty}))(a|\epsilon)^{0,3}) \big) = \\[-0.2em]
        & \quad\quad\quad\quad (1,\{1\}, (2,\{2,3\},(0,\emptyset,\epsilon) \mid (0,\emptyset,(0,\emptyset,a)^{0,\infty})) \\[-0.2em]
        & \quad\quad\quad\quad\quad\quad\enspace \cdot (3,\emptyset,(4,\{4\},(0,\emptyset,a) \mid (0,\emptyset,\epsilon))^{0,3}))
    \end{aligned}$
    }};
\end{scope}

\newcommand\xsp[1]{\hphantom{\hspace{#1em}\hspace{0.2em}}}

\begin{scope}[xshift=3in, yshift=-0.1in, sibling distance=0.6in, level distance=0.35in]
    \graph [tree layout, grow=down, fresh nodes] {
        a1/"${T}^{1}_{\Lambda}$" -- {
            a11/"${T}^{2}_{1}$" -- {
                a111/"${\bot}^{0}_{1.1}$",
                a112/"${T}^{0}_{1.2}$" -- {
                    a1121/"${a}^{0}_{1.2.1}$"
                }
            },
            a12/"${T}^{3}_{2}$" -- {
                a121/"${\bot}^{4}_{2.1}$"
            }
        }
    };
    \node at (a1)    {\xsp{2.5}\footnotesize{$(1)$}};
    \node at (a11)   {\xsp{2.5}\footnotesize{$(1)$}};
    \node at (a111)  {\xsp{3.5}\footnotesize{$(\infty)$}};
    \node at (a112)  {\xsp{3.5}\footnotesize{$(\infty)$}};
    \node at (a1121) {\xsp{4.0}\footnotesize{$(\infty)$}};
    \node at (a12)   {\xsp{2.5}\footnotesize{$(0)$}};
    \node at (a121)  {\xsp{3.0}\footnotesize{$(-1)$}};

    \node[xshift=0in, yshift=-1.35in, draw=none]
    {$s \;=\; {T}^{1} (
        {T}^{2} (
            {\bot}^{0},
            {T}^{0}({a}^{0})
        ),
        {T}^{3}(
            {\bot}^{4}
        )
    )$};
\end{scope}

\begin{scope}[xshift=3in, yshift=-1.9in, sibling distance=0.6in, level distance=0.35in]
    \graph [tree layout, grow=down, fresh nodes] {
        a1/"${T}^{1}_{\Lambda}$" -- {
            a11/"${T}^{2}_{1}$" -- {
                a111/"${\epsilon}^{0}_{1.1}$",
                a112/"${\bot}^{0}_{1.2}$"
            },
            a12/"${T}^{3}_{2}$" -- {
                a121/"${T}^{4}_{2.1}$" -- {
                    a1211/"${a}^{0}_{2.1.1}$",
                    a1212/"${\bot}^{0}_{2.1.2}$"
                },
                a122/"${T}^{4}_{2.2}$" -- {
                    a1221/"${\bot}^{0}_{2.2.1}$",
                    a1222/"${\epsilon}^{0}_{2.2.2}$"
                }
            }
        }
    };
    \node at (a1)    {\xsp{2.5}\footnotesize{$(1)$}};
    \node at (a11)   {\xsp{2.5}\footnotesize{$(0)$}};
    \node at (a111)  {\xsp{3.5}\footnotesize{$(\infty)$}};
    \node at (a112)  {\xsp{3.5}\footnotesize{$(\infty)$}};
    \node at (a12)   {\xsp{2.5}\footnotesize{$(1)$}};
    \node at (a121)  {\xsp{3.0}\footnotesize{$(1)$}};
    \node at (a1211) {\xsp{3.5}\footnotesize{$(\infty)$}};
    \node at (a1212) {\xsp{3.5}\footnotesize{$(\infty)$}};
    \node at (a122)  {\xsp{3.0}\footnotesize{$(0)$}};
    \node at (a1221) {\xsp{3.5}\footnotesize{$(\infty)$}};
    \node at (a1222) {\xsp{3.5}\footnotesize{$(\infty)$}};

    \node[xshift=0in, yshift=-1.35in, draw=none]
    {$r \;=\; {T}^{1}(
        {T}^{2}(
            {\epsilon}^{0},
            {\bot}^{0}
        ),
        {T}^{3}(
            {T}^{4}({a}^{0},{\bot}^{0}),
            {T}^{4}({\bot}^{0}, {\epsilon}^{0})
        )
    )$};
\end{scope}

\begin{scope}[xshift=3in, yshift=-3.7in, sibling distance=0.6in, level distance=0.35in]
    \graph [tree layout, grow=down, fresh nodes] {
        a1/"${T}^{1}_{\Lambda}$" -- {
            a11/"${T}^{2}_{1}$" -- {
                a111/"${\bot}^{0}_{1.1}$",
                a112/"${T}^{0}_{1.2}$" -- {
                    a1121/"${\bot}^{0}_{1.2.1}$"
                }
            },
            a12/"${T}^{3}_{2}$" -- {
                a121/"${T}^{4}_{2.1}$" -- {
                    a1211/"${a}^{0}_{2.1.1}$",
                    a1212/"${\bot}^{0}_{2.1.2}$"
                }
            }
        }
    };
    \node at (a1)    {\xsp{2.5}\footnotesize{$(1)$}};
    \node at (a11)   {\xsp{2.5}\footnotesize{$(0)$}};
    \node at (a111)  {\xsp{3.5}\footnotesize{$(\infty)$}};
    \node at (a112)  {\xsp{3.5}\footnotesize{$(\infty)$}};
    \node at (a1121) {\xsp{4.0}\footnotesize{$(\infty)$}};
    \node at (a12)   {\xsp{2.5}\footnotesize{$(1)$}};
    \node at (a121)  {\xsp{3.0}\footnotesize{$(1)$}};
    \node at (a1211) {\xsp{3.5}\footnotesize{$(\infty)$}};
    \node at (a1212) {\xsp{3.5}\footnotesize{$(\infty)$}};

    \node[xshift=-0in, yshift=-1.35in, draw=none]
    {$t \;=\; {T}^{1}(
        {T}^{2}(
            {\bot}^{0},
            {T}^{0}({\bot}^{0})
        ),
        {T}^{3}(
            {T}^{4}({a}^{0},{\bot}^{0})
        )
    )$};
\end{scope}
}

\end{tikzpicture}

\end{document}

